Shallow/SeqDiskProg.v
@@ -16,7 +16,7 @@ Module D.
 
   Inductive step : Semantics Op State :=
   | step_read : forall a b state,
-      (forall b0, diskMem (sdisk state) a = Some b0 -> b = b0) ->
+      (forall b0, sdisk state a = Some b0 -> b = b0) ->
       step (Read a) state b state
   | step_write : forall a b state,
       step (Write a b) state tt (Disk (diskUpd (sdisk state) a b)).
